organization

SampCert/DifferentialPrivacy/Queries/UnboundedMax/Properties.lean
@@ -16,6 +16,30 @@ noncomputable section
 
 namespace SLang
 
+
+/-
+# Util
+-/
+
+/--
+Simpler bijection lemma which ignores the support (makes for much easier fn definitions)
+-/
+lemma tsum_eq_tsum_of_bij {α : Type u_1} {β : Type u_2} {γ : Type u_3} [AddCommMonoid α]
+  [TopologicalSpace α] {f : β → α} {g : γ → α}
+    (i : γ → β)
+    (hi : Function.Injective i)
+    (hf : Function.support f ⊆ Set.range fun (x : ↑(Function.support g)) => i ↑x)
+    (hfg : ∀ (x : γ), f (i x) = g x) :
+  ∑' (x : β), f x = ∑' (y : γ), g y := by
+  apply tsum_eq_tsum_of_ne_zero_bij (fun x => i x)
+  · simp [Function.Injective]
+    exact fun a _ a_1 _ a_2 => hi a_2
+  · trivial
+  · simp_all
+
+
+
+
 /-
 ## Abstract sparse vector mechanism code
 -/
@@ -214,28 +238,97 @@ theorem gen_sv_loop_cut_eventually_constant_true_false (cond : List ℤ -> Bool)
     sorry
 
 
+/--
+After a threshold, probWhileCut gen_sv_cond (gen_sv_body cond noise) is constant in terms of the amount of fuel.
+-/
+def gen_sv_loop_cut_step (cond : List ℤ -> Bool) (noise : SLang ℤ) (fuel : ℕ) (init : List ℤ) : SLang (Bool × List ℤ) :=
+  (fun (eval_f, eval) =>
+    match eval_f with
+    | true => 0 -- What is the true->true closed form?
+    | false =>
+        -- true->false closed form: Either there is not enough iterates to reach the eval point, so the
+        -- probability is zero, or there is enough, and the probability is constant.
+        if fuel < eval.length - init.length
+          then 0
+          else probWhileCut gen_sv_cond (gen_sv_body cond noise) (eval.length - init.length) (true, init) (false, eval))
+
+
+theorem gen_sv_loop_closed (cond : List ℤ -> Bool) (noise : SLang ℤ) (fuel : ℕ) (init : List ℤ) :
+    probWhileCut gen_sv_cond (gen_sv_body cond noise) fuel (true, init)  =
+    gen_sv_loop_cut_step cond body fuel init := by
+  sorry
+
+
+/--
+History-tracking sparse-vector mechanism
+-/
+def gen_sv_num (cond : List ℤ -> Bool) (noise : SLang ℤ) : SLang ℕ :=
+  gen_sv cond noise >>= (probPure ∘ List.length)
+
+/--
+Sparse vector mechanism which calculates each point using a fixed number of iterates
+-/
+def gen_sv_num_cut (cond : List ℤ -> Bool) (noise : SLang ℤ) : SLang ℕ :=
+  fun N => (gen_sv_cut cond noise (N + 1) (true, []) >>= (probPure ∘ List.length)) N
+
+/-
+## Reduction 1: Unbounded compilable program to bounded noncompilable program
+-/
+
+lemma gen_sv_reduction_1 cond noise : gen_sv_num cond noise = gen_sv_num_cut cond noise := by
+  -- Prove that gen_sv_num_cut is constant after N iterates
+  -- Apply the limit lemma
+  sorry
 
 
 
 /-
-Reduction 1: Unbounded compilable program to bounded noncompilable program
+## Reduction 2: Bounded noncompilable program to Presampled program
 -/
+
+
+def gen_sv_presampleN (noise : SLang ℤ) (N : ℕ) : SLang (List ℤ) :=
+  match N with
+  | Nat.zero => probPure []
+  | Nat.succ N' => do
+      let vN' <- noise
+      let rec <- gen_sv_presampleN noise N'
+      return rec ++ [vN']
+
+lemma gen_sv_presampleN_supp (noise : SLang ℤ) (N : ℕ) (eval : List ℤ) :
+    gen_sv_presampleN noise N eval ≠ 0 -> eval.length = N := by
+  sorry
+
+
+/--
+Conditionals which are monotone
+-/
+def cond_mono_pred (cond : List ℤ -> Bool) : Prop :=
+  ∀ l d : List ℤ, cond l = false -> cond (l ++ d) = false
+
+/--
+Sparse vector mechanism which calculates randomness ahead of time and
+only checks one point
+-/
+def gen_sv_presampled (cond : List ℤ -> Bool) (noise : SLang ℤ) : SLang ℕ :=
+  fun N =>
+  (gen_sv_presampleN noise N >>= fun hist =>
+   noise >>= fun last =>
+   if (¬ cond (hist ++ [last]) ∧ cond hist)
+     then probPure N
+     else 0)
+  N
+
+lemma gen_sv_reduction_2 (cond : List ℤ -> Bool) (noise : SLang ℤ) (Hcond : cond_mono_pred cond) :
+  gen_sv_num_cut cond noise = gen_sv_presampled cond noise := by
+  sorry
+
 
 
 /-
-Reduction 2: Bounded noncompilable program to Presampled program
+## Specialization to the terms used for privMax
 -/
 
-
-
-
-
-
-
-
-/-
-# Concrete program, used in the pure DP proof
--/
 
 
 
@@ -269,7 +362,6 @@ lemma G_mono (l : List ℕ) (vis : { v : List ℤ // 0 < v.length }) (c : ℤ) p
   trivial
 
 
-
 /--
 History-aware loop condition for the privMax program
 -/
@@ -279,1353 +371,21 @@ def privMax_eval_alt_cond (l : List ℕ) (τ : ℤ) (history : List ℤ) : Bool 
   | (h :: hs) => G l ⟨ h :: hs , by simp ⟩ < τ
 
 
-
-
-
-
-
-
-
-
-
-
-
-
-
-
-
-
-
-
-
-
-
-
-
-
-
-
-
-
-
-
-
-
-
-
-
-
-
-
-
-
-
-
-
-
-
-
-
-
-
-
-
-/-
-# Loop unrolling lemmas
-
-`probWhileSplit cond body continuation n` is an n-unrolling of a loop, where `continuation` is
-      applied in the case that n is exhaused.
-
-`probWhileCut cond body n` is a `probWhileSplit` with continuation zero.
-
-`probWhileSplit .. continuation (m + n)` is the same as `probWhileSplit .. .. m` with a
-    `probWhileSplit .. continuation n` continuation.
-
-`probWhileSplit .. probPure (m + n)`  is the same as `probWhileSplit .. probPure m` bound to
-    `probWhileSplit .. probPure b`.
-
-`probWhileSplit .. probZero (m + n)`  is the same as `probWhileSplit .. probPure m` bound to
-    `probWhileSplit .. probZero b`, provided `n > 0`. This last lemma enables us to separate
-    the first m unrollings of a nontrivial probWhile loop.
-
-The helper function `probBind_congr_strong` enables us to restruct congruence proofs between
-    probBind programs to their support.
-
-The predicate
--/
-
 /--
-Stronger congruence rule for probBind: The bound-to functions have to be equal only on the support of
-the bound-from function.
+Compute privMax with presampling
 -/
-lemma probBind_congr_strong (p : SLang T) (f : T -> SLang U) (g : T -> SLang U) (Hcong : ∀ t : T, p t ≠ 0 -> f t = g t) :
-    p >>= f = p >>= g := by
-  simp
-  unfold probBind
-  apply SLang.ext
-  intro u
-  apply Equiv.tsum_eq_tsum_of_support ?G1
-  case G1 =>
-    apply Set.BijOn.equiv (fun x => x)
-    simp [Function.support]
-    have Heq : {x | ¬p x = 0 ∧ ¬f x u = 0} =  {x | ¬p x = 0 ∧ ¬g x u = 0} := by
-      apply Set.sep_ext_iff.mpr
-      intro t Ht
-      rw [Hcong]
-      apply Ht
-    rw [Heq]
-    apply Set.bijOn_id
-  simp [Function.support]
-  intro t ⟨ Hp, _ ⟩
-  simp [Set.BijOn.equiv]
-  rw [Hcong]
-  apply Hp
-
-lemma probBind_congr_medium (p : SLang T) (f : T -> SLang U) (g : T -> SLang U) (u : U)
-      (Hcong : ∀ t : T, p t ≠ 0 -> f t u = g t u) :
-      (p >>= f) u = (p >>= g) u := by
-   simp
-   apply Equiv.tsum_eq_tsum_of_support ?G1
-   case G1 =>
-     apply Set.BijOn.equiv (fun x => x)
-     simp [Function.support]
-     have Heq : {x | ¬p x = 0 ∧ ¬f x u = 0} =  {x | ¬p x = 0 ∧ ¬g x u = 0} := by
-       apply Set.sep_ext_iff.mpr
-       intro t Ht
-       rw [Hcong]
-       apply Ht
-     rw [Heq]
-     apply Set.bijOn_id
-   simp [Function.support]
-   intro t ⟨ Hp, _ ⟩
-   simp [Set.BijOn.equiv]
-   rw [Hcong]
-   apply Hp
-
-
-/--
-``SLang`` value obtained by applying a loop body exactly ``n`` times to a given distribution
--/
-def probWhileSplit (cond : T → Bool) (body : T → SLang T) (continuation : T -> SLang T) (n : Nat) (a : T) : SLang T :=
-  match n with
-  | Nat.zero => continuation a
-  | Nat.succ n => do
-    if cond a
-      then
-        let v ← body a
-        probWhileSplit cond body continuation n v
-      else
-        return a
-
-
-/--
-probWhileCut is probWhileSplit applied to the zero distribution
--/
-lemma probWhileCut_probWhileSplit_zero (cond : T → Bool) (body : T → SLang T) (n : Nat) :
-    probWhileCut cond body n = probWhileSplit cond body (fun _ => probZero) n := by
-  apply funext
-  induction n
-  · simp [probWhileCut, probWhileSplit]
-  · rename_i n IH
-    simp [probWhileCut, probWhileSplit]
-    rw [funext IH]
-    intro _
-    rfl
-
-/--
-Evaluate probWhileSplit when out of steps
--/
-lemma probWhileSplit_zero (cond : T → Bool) (body : T → SLang T) (continuation : T -> SLang T) (init : T):
-    probWhileSplit cond body continuation 0 init = continuation init := by
-  simp [probWhileSplit]
-
-/--
-probWhileSplit is constant when the condition is false
--/
-lemma probWhileSplit_cond_false_cst (cond : T → Bool) (body : T → SLang T) (continuation : T -> SLang T)
-    (n : Nat) (init : T) (HF : cond init ≠ true) :
-    probWhileSplit cond body continuation (Nat.succ n) init =
-    probPure init := by
-  rw [probWhileSplit]
-  split
-  · exfalso
-    simp_all
-  rfl
-
-/--
-Move an iterate of of probWhileSplit into the continuation.
--/
-lemma probWhileSplit_succ_l (cond : T → Bool) (body : T → SLang T) (continuation : T -> SLang T) (n : Nat) (init : T):
-    probWhileSplit cond body continuation (Nat.succ n) init =
-    (probWhileSplit cond body (probWhileSplit cond body continuation n) 1 init) := by
-  apply funext
-  intro _
-  simp [probWhileSplit]
-
-/--
-Move multiple iterates of of probWhileSplit into the continuation.
--/
-lemma probWhileSplit_add_l (cond : T → Bool) (body : T → SLang T) (continuation : T -> SLang T) (m n : Nat) (init : T):
-    probWhileSplit cond body continuation (n + m) init =
-    (probWhileSplit cond body (probWhileSplit cond body continuation n) m init) := by
-  revert init
-  induction m
-  · intro init
-    rw [probWhileSplit_zero]
-    simp only [add_zero]
-  · intro init
-    rename_i m' IH
-    rw [probWhileSplit_succ_l]
-    rw [<- (funext IH)]
-    rw [<- probWhileSplit_succ_l]
-    rfl
-
-
-/--
-Move iterate of probWhileSplit into the initial value, when the continuation is probPure
--/
-lemma probWhileSplit_succ_r_pure (cond : T → Bool) (body : T → SLang T) (n : Nat) (init : T):
-    probWhileSplit cond body probPure (Nat.succ n) init =
-    (probWhileSplit cond body probPure 1 init)  >>=  (probWhileSplit cond body probPure n) := by
-  apply funext
-  intro x
-  have H : (probWhileSplit cond body probPure 1 init) = if (cond init) then (body init) >>= probPure else pure init := by
-    apply funext
-    intro x
-    rw [probWhileSplit]
-    split
-    · simp [probWhileSplit]
-    · rfl
-  rw [H]
-  simp only [probWhileSplit]
-  split
-  · simp
-  · have H : (pure init >>= probWhileSplit cond body probPure n) = pure init := by
-      apply funext
-      intro x
-      simp [pure_apply]
-      conv =>
-        lhs
-        enter [1, a]
-      rw [ENNReal.tsum_eq_add_tsum_ite init]
-      simp
-      cases n
-      · simp [probWhileSplit]
-        rw [ENNReal.tsum_eq_zero.mpr ?G1]
-        case G1 =>
-          intro i
-          split <;> rfl
-        simp
-      · rename_i n'
-        rw [probWhileSplit_cond_false_cst _ _ _ _ _ (by trivial)]
-        simp [probPure]
-        rw [ENNReal.tsum_eq_zero.mpr ?G1]
-        case G1 =>
-          intro i
-          split <;> rfl
-        simp
-    rw [H]
-
-
-/--
-Move iterates of probWhileSplit into the initial value, when the continuation is probPure
--/
-lemma probWhileSplit_add_r_pure (cond : T → Bool) (body : T → SLang T) (m n : Nat) (init : T):
-    probWhileSplit cond body probPure (m + n) init =
-    (probWhileSplit cond body probPure m init)  >>=  (probWhileSplit cond body probPure n) := by
-  revert init
-  induction m
-  · simp [probWhileSplit]
-  · intro init
-    rename_i m' IH
-    rw [add_comm, <- add_assoc]
-    rw [probWhileSplit_succ_r_pure]
-    rw [add_comm]
-    rw [bind_congr IH]
-    rw [probWhileSplit_succ_r_pure _ _ m']
-    conv =>
-      congr
-      · enter [1]
-        simp [probWhileSplit]
-      · enter [1, 1]
-        simp [probWhileSplit]
-    split <;> simp
-
-
-
-
-/--
-Move iterate of probWhileSplit into initial condition, when continuation is probZero
--/
-lemma probWhileSplit_succ_r_zero (cond : T → Bool) (body : T → SLang T) (n : Nat) (Hn : n > 0) (init : T):
-    probWhileSplit cond body (fun _ => probZero) (Nat.succ n) init =
-    (probWhileSplit cond body probPure 1 init)  >>=  (probWhileSplit cond body (fun _ => probZero) n) := by
-  apply funext
-  intro x
-  simp [probWhileSplit]
-  split
-  · simp [probBind]
-  · rename_i h
-    simp at h
-    conv =>
-      rhs
-      enter [1, a]
-      simp [probPure]
-    rw [ENNReal.tsum_eq_add_tsum_ite init]
-    simp
-    have H1 :
-      (∑' (x_1 : T), if x_1 = init then 0 else if x_1 = init then probWhileSplit cond body (fun _ => probZero) n x_1 x else 0) = 0 := by
-      apply ENNReal.tsum_eq_zero.mpr
-      intro i
-      split <;> simp
-    simp [H1]
-    clear H1
-    unfold probWhileSplit
-    cases n
-    · exfalso
-      linarith
-    · simp [h]
-
-
-/--
-Move iterate of probWhileSplit into initial condition, when continuation is probZero
--/
-lemma probWhileSplit_add_r_zero (cond : T → Bool) (body : T → SLang T) (m n : Nat) (Hn : n > 0) (init : T):
-    probWhileSplit cond body (fun _ => probZero) (m + n) init =
-    (probWhileSplit cond body probPure m init)  >>=  (probWhileSplit cond body (fun _ => probZero) n) := by
-  revert init
-  induction m
-  · intro init
-    simp [probWhileSplit]
-  · intro init
-    rename_i m' IH
-    conv =>
-      lhs
-      rw [add_comm, <- add_assoc]
-    rw [probWhileSplit_succ_r_zero _ _ _ (by linarith)]
-    rw [add_comm]
-    cases m'
-    · simp
-    rename_i m''
-    rw [bind_congr IH]
-    clear IH
-    unfold probWhileSplit
-    simp
-    split <;> simp
-    · rename_i h
-      apply probBind_congr_strong
-      intro t _
-      simp [probWhileSplit]
-    · rw [if_neg (by trivial)]
-      simp
-
-/--
-Separate out the first m unrollings of a nontrivial probWhileCut loop
--/
-theorem probWhileCut_add_r (cond : T → Bool) (body : T → SLang T) (m n : Nat) (Hn : n > 0) (init : T):
-    probWhileCut cond body (m + n) init =
-    (probWhileSplit cond body probPure m init) >>= (probWhileCut cond body n) := by
-  rw [probWhileCut_probWhileSplit_zero]
-  rw [probWhileCut_probWhileSplit_zero]
-  apply probWhileSplit_add_r_zero
-  trivial
-
-
-
-lemma unfunext (f g : A -> B) (a : A) (H : f = g) : f a = g a := by
-  subst H
-  rfl
-
-
--- /--
--- Probability that loop terminates using exactly N successful evaluations of the loop head
--- -/
--- def probTermCut (cond : T → Bool) (body : T → SLang T) (N : ℕ) (init : T) : SLang Bool :=
---   match N with
---   | Nat.zero =>
---     -- Have done N successes at the loop head, next loop head must fail
---     if cond init
---       then probPure False
---       else probPure True
---   | Nat.succ N' =>
---     -- Haven't done N successes at the loop head, next loop head must succeed
---     if cond init
---       then (body init) >>= (probTermCut cond body N')
---       else probPure False
---
---
--- /--
--- Probability mass at each point associated only to loop iterates that terminate in N steps
--- -/
--- def indicTermN (cond : T → Bool) (body : T → SLang T) (N : ℕ) (init : T) : SLang T := do
---   let tN <- probTermCut cond body N init
---   if tN
---     then probWhileSplit (fun _ => true) body probPure N init
---     else probZero
---
---
--- lemma probWhileCut_indic_ind (cond : T → Bool) (body : T → SLang T) (N : ℕ) (init : T) (eval : T) :
---   probWhileCut cond body (N + 1) init eval = probWhileCut cond body N init eval + indicTermN cond body N init eval := by
---   simp [indicTermN]
---   rw [tsum_bool]
---   simp
---
---   sorry
-  -- revert init eval
-  -- induction N
-  -- · intro init eval
-  --   simp [probWhileCut, probWhileFunctional]
-  --   simp [indicTermN, probTermCut]
-  --   rw [tsum_bool]
-  --   split <;> simp [probWhileSplit]
-  -- · intro init eval
-  --   rename_i N' IH
-  --   rw [probWhileCut_probWhileSplit_zero]
-  --   rw [probWhileSplit_add_l]
-  --   rw [<- probWhileCut_probWhileSplit_zero]
-  --   have IH' : probWhileCut cond body (N' + 1) = (fun init eval => probWhileCut cond body N' init eval + indicTermN cond body N' init eval) := by
-  --     apply funext
-  --     intro init'
-  --     apply funext
-  --     intro eval'
-  --     apply IH init' eval'
-  --   simp [probWhileSplit]
-  --   split
-  --   · sorry
-  --   · simp [probWhileCut, probWhileFunctional]
-  --     simp [indicTermN]
-  --     sorry
-
-
-
--- lemma probWhileCut_indic_sum (cond : T → Bool) (body : T → SLang T) (N : ℕ) (init : T) (eval : T) :
---   probWhileCut cond body N init eval = ∑'(i : ℕ), if i < N then (indicTermN cond body i init) eval else 0 := by
---   induction N
---   · simp [probWhileCut]
---   rename_i N' IH
---   sorry
-
-
-
-
-
-
-
-
-
-
-
-
-
-
-
-
-
-
-
-
-
-
-
-
-
-
-
-
-/-
-
-/--
-Once a history terminates the loop, any hypothetical future loop conditions are also aware that it terminates
--/
-lemma privMax_G_continue_alt_mono (l : List ℕ) (τ : ℤ) (history : List ℤ) (future : ℤ) :
-    ¬ privMax_eval_alt_cond l τ history -> ¬ privMax_eval_alt_cond l τ (history ++ [future]):= by
-  unfold privMax_eval_alt_cond
-  cases history
-  · simp
-  rename_i a b
-  simp only [decide_eq_true_eq, List.cons_append]
-  intro H1 H2
-  apply H1
-  apply LE.le.trans_lt _ H2
-  apply G_mono
-
-
-
-/--
-History-aware body for the privMax sampling loop
--/
-def privMax_eval_alt_F {dps : DPSystem ℕ} (ε₁ ε₂ : ℕ+) (history : List ℤ) : SLang (List ℤ) := do
-  let candidate <- @privNoiseZero dps ε₁ (4 * ε₂)
-  return history ++ [candidate]
-
-
-
-/--
-Support of privMaxEval_alt_body is contained in the extensions of the history by one element
--/
-lemma privMaxEval_alt_body_supp {dps : DPSystem ℕ} (ε₁ ε₂ : ℕ+) history eval :
-    (@privMax_eval_alt_F dps ε₁ ε₂ history eval) ≠ 0 -> ∃ z, eval = history ++ [z] := by
-  simp [privMax_eval_alt_F ]
-  intro x Heval _
-  exists x
-
--- FIXME: cleanup proof
-lemma privMaxEval_alt_body_supp' {dps : DPSystem ℕ} (ε₁ ε₂ : ℕ+) history eval :
-    (¬(∃ z, eval = history ++ [z])) -> (@privMax_eval_alt_F dps ε₁ ε₂ history eval) = 0 := by
-  apply Classical.by_contradiction
-  intro A
-  apply A
-  intro B
-  suffices ¬(privMax_eval_alt_F ε₁ ε₂ history eval ≠ 0) by
-    exact False.elim (this fun a => A fun _ => a)
-  intro C
-  apply B
-  apply privMaxEval_alt_body_supp ε₁ ε₂
-  trivial
-
-
-def privMax_eval_alt_loop {dps : DPSystem ℕ} (ε₁ ε₂ : ℕ+) (l : List ℕ) (τ : ℤ) : SLang (List ℤ) := do
-  probWhile
-    (privMax_eval_alt_cond l τ)
-    (@privMax_eval_alt_F dps ε₁ ε₂)
-    []
-
-
-/--
-History-aware privMax program
--/
-def privMax_eval_alt {dps : DPSystem ℕ} (ε₁ ε₂ : ℕ+) (l : List ℕ) : SLang ℕ := do
+def privMax_presample {dps : DPSystem ℕ} (ε₁ ε₂ : ℕ+) (l : List ℕ) : SLang ℕ := do
   let τ <- @privNoiseZero dps ε₁ (2 * ε₂)
-  let final_history <- @privMax_eval_alt_loop dps ε₁ ε₂ l τ
-  return final_history.length - 1
-
-/-
-## Reduction 0: The implementation version is the same as the history-tracking version
+  gen_sv_presampled (privMax_eval_alt_cond l τ) (@privNoiseZero dps ε₁ (4 * ε₂))
 
 
-This reduction is not necessary, technically, since privMax_eval_alt is computable.
-The later reductions, on the other hand, are necessary.
--/
-
-lemma privMax_reduction_0 (ε₁ ε₂ : ℕ+) (l : List ℕ) :
-    @privMax_eval dps ε₁ ε₂ l = @privMax_eval_alt dps ε₁ ε₂ l := by
-  unfold privMax_eval privMax_eval_alt
-  simp
-  apply funext
-  intro N
-  simp
-  apply tsum_congr
-  intro τ
-  congr 1
-  unfold privMax_eval_alt_loop
-  conv =>
-    enter [1, 1, a, 2]
-    rw [ENNReal.tsum_prod']
-
-  -- Separate the sum on the right into a sum over list lengths?
+lemma privMax_presample_normalizes {dps : DPSystem ℕ} (ε₁ ε₂ : ℕ+) (l : List ℕ) : HasSum (@privMax_presample dps ε₁ ε₂ l) 1 := by
   sorry
 
-
-
-
-/-
-## Reduction 1: The history-tracking version is the same as a bounded history-tracking version
--/
-
-
 /--
-Sampling loop for the bounded history-aware privMax function
-
-Truncated to N iterates; stable for all lists of length at most N-1
+privMax as a PMF
 -/
-def privMax_eval_alt_loop_cut {dps : DPSystem ℕ} (ε₁ ε₂ : ℕ+) (l : List ℕ) (τ : ℤ) (N : ℕ) : SLang (List ℤ) := do
-  probWhileCut
-    (privMax_eval_alt_cond l τ)
-    (@privMax_eval_alt_F dps ε₁ ε₂)
-    N
-    []
-
-/--
-Closed form for privMax_eval_alt_loop_cut evaluated on the history hist, in terms of the number of iterates.
-
-Namely, it is a step function. The function probWhileCut needs (hist.length + 1) iterates before hist
-is in its support, and afterwards, no additional iterates return hist.
--/
-def privMax_eval_alt_loop_cut_step {dps : DPSystem ℕ} (ε₁ ε₂ : ℕ+) (l : List ℕ) (τ : ℤ) (iterates : ℕ) (hist : List ℤ) : ENNReal :=
-  if (iterates ≤ hist.length)
-    then 0
-    else probWhileCut (privMax_eval_alt_cond l τ) (@privMax_eval_alt_F dps ε₁ ε₂) (hist.length + 1) [] hist
-
-
-/--
-Length of the supported region is bounded below by the length of the initial history.
--/
-lemma privMax_eval_cut_supp_bound {dps : DPSystem ℕ} (ε₁ ε₂ : ℕ+) (C : List ℤ -> Bool) (A B : List ℤ)
-  (HAB : A.length > B.length) :
-    probWhileCut C (@privMax_eval_alt_F dps ε₁ ε₂) N A B = 0 := by
-  revert A
-  induction N
-  · simp [probWhileCut]
-  · intro A HA
-    rename_i N' IH
-    simp [probWhileCut, probWhileFunctional]
-    split
-    · simp
-      intro F_A
-      cases Classical.em (∃ z : ℤ, F_A = A ++ [z])
-      · rename_i h
-        rcases h with ⟨ z, HF_A ⟩
-        right
-        apply IH
-        simp [HF_A]
-        linarith
-      · left
-        apply privMaxEval_alt_body_supp'
-        trivial
-    · simp
-      intro HK
-      simp [HK] at HA
-
-
-
-
-
-
-/--
-Length of supported region is bounded abouve by the length of the initial history, plus the number of iterations.
--/
-lemma privMax_eval_cut_supp_bound' {dps : DPSystem ℕ} (ε₁ ε₂ : ℕ+) (C : List ℤ -> Bool) (A B : List ℤ)
-    (HAB : A.length + N < B.length + 1) :
-    probWhileCut C (@privMax_eval_alt_F dps ε₁ ε₂) N A B = 0 := by
-  revert A
-  induction N
-  · intro _ _
-    simp [probWhileCut]
-  · intro A HA
-    rename_i N' IH
-    simp [probWhileCut, probWhileFunctional]
-    split
-    · simp
-      intro F_A
-      cases Classical.em (∃ z : ℤ, F_A = A ++ [z])
-      · rename_i h
-        rcases h with ⟨ z, HF_A ⟩
-        right
-        apply IH
-        simp [HF_A]
-        linarith
-      · left
-        apply privMaxEval_alt_body_supp'
-        trivial
-    · simp
-      intro HK
-      simp [HK] at HA
-
--- TODO: Can I prove strong congruence for the constant true split?
-
-
--- TODO: Can I prove support for the constant true split?
-
-
--- lemma privMax_eval_const_true_supp_spec {dps : DPSystem ℕ} (ε₁ ε₂ : ℕ+) (cont : List ℤ -> SLang (List ℤ)) (A B : List ℤ) (N : ℕ)
---     (HContSupp : ∀ C D : List ℤ, C.length < D.length + 1 -> cont C D = 0) (H : A.length + N < B.length + 1) :
---     probWhileSplit (fun _ => True) (@privMax_eval_alt_F dps ε₁ ε₂) cont N A B = 0 := by
---   revert A
---   induction N
---   · intro A HA
---     simp [probWhileSplit]
---     apply HContSupp
---     simp_all
---   · intro A HA
---     rename_i n' IH
---     simp [probWhileSplit]
---     intro F_A
---     cases Classical.em (∃ z : ℤ, F_A = A ++ [z])
---     · right
---       rename_i h
---       rcases h with ⟨ z, Hz ⟩
---       subst Hz
---       apply IH
---       simp
---       linarith
---     · left
---       apply privMaxEval_alt_body_supp'
---       trivial
---
---
---
--- -- Effectively circular due to the side condition constraint on ConstSupp?
--- lemma privMax_eval_split_supp_bound' {dps : DPSystem ℕ} (ε₁ ε₂ : ℕ+) (C : List ℤ -> Bool)
---     (cont : List ℤ -> SLang (List ℤ)) (B : List ℤ)
---     (HContSupp : ∀ (C D : List ℤ), C.length < D.length + 1 → cont C D = 0)
---     (HB : A.length + N < B.length + 1) :
---     probWhileSplit C (@privMax_eval_alt_F dps ε₁ ε₂) cont N A B =
---     probWhileSplit (fun _ => True) (@privMax_eval_alt_F dps ε₁ ε₂) cont N A B := by
---   revert A
---   induction N
---   · intro _ _
---     simp [probWhileSplit]
---   · intro A HA
---     rename_i N' IH
---     simp only [probWhileSplit, decide_True, ↓reduceIte]
---     split
---     · apply probBind_congr_medium
---       intro A' HA'
---       apply IH
---       apply privMaxEval_alt_body_supp at HA'
---       rcases HA' with ⟨ z, hz ⟩
---       subst hz
---       simp
---       linarith
---     · conv =>
---         lhs
---         simp
---       split
---       · exfalso
---         rename_i HK
---         subst HK
---         simp at HA
---       symm
---       simp
---       intro F_A
---       cases Classical.em (∃ z : ℤ, F_A = A ++ [z])
---       · rename_i h
---         rcases h with ⟨ z, Hz ⟩
---         subst Hz
---         right
---         -- After the N' iterates, the length of F(F(F(...(F(A ++ [z]))))) is A.length + N' + 1
---         -- This length is less than B + 1 by hyp.
---         -- So, applying the contniuation support property, it is zero.
---         apply privMax_eval_const_true_supp_spec
---         · trivial
---         · simp
---           linarith
---       · left
---         apply privMaxEval_alt_body_supp'
---         trivial
-
-
-/--
-Test lemma: privMax loop cut equals its closed form at []
--/
-lemma privMax_eval_alt_loop_cut_closed_base {dps : DPSystem ℕ} :
-    @privMax_eval_alt_loop_cut dps ε₁ ε₂ l τ N [] = @privMax_eval_alt_loop_cut_step dps ε₁ ε₂ l τ N [] := by
-  simp [privMax_eval_alt_loop_cut]
-
-  cases N
-  · -- For N = 0 we are below the step
-    -- Simplify the RHS. Below the step, so it is constant 0.
-    conv =>
-      rhs
-      simp [privMax_eval_alt_loop_cut_step]
-    -- Simplify the LHS. There are not enough steps (0 ≤ [].length) so it is 0.
-    conv =>
-      lhs
-      simp [probWhileCut]
-  · -- For N ≥ 1 we are above the step
-    rename_i N'
-    -- Simplify the RHS. Above the step, so it is probWhilecut _ _ ([].length + 1) [] []
-    conv =>
-      rhs
-      simp [privMax_eval_alt_loop_cut_step]
-    -- Separate the first iterate from both sides.
-    -- Have to handle special case where N' = 0 and the formula doesn't hold
-    cases N'
-    · simp
-    rename_i N''
-    rw [probWhileCut_probWhileSplit_zero,
-        probWhileCut_probWhileSplit_zero]
-    rw [add_comm]
-    rw [probWhileSplit_add_r_zero _ _ _ _ ?G1]
-    case G1 => simp
-
-    -- rewrite the RHS to a bind
-
-    -- Either the bound-from term will do:
-    --  early return, so false forever
-    --  continuation, with so much context that the RHS is false forever
-
-
-
-
-
-    sorry
-
-
-
-
-
-
-
-
-
-
-
-
-
-
-
-
-
-
-
-
-
-
-
-
-
-/--
-After a certain number of iterations, the function stops changing.
--/
-lemma privMax_eval_cut_const_ind {dps : DPSystem ℕ} (ε₁ ε₂ : ℕ+) (C : List ℤ -> Bool) (B : List ℤ)
-    (HN : B.length + 1 ≤ N) :
-    probWhileCut C (@privMax_eval_alt_F dps ε₁ ε₂) N [] B =
-    probWhileCut C (@privMax_eval_alt_F dps ε₁ ε₂) (N + 1) [] B := by
-
-  -- We should be able to prove this by rewriting into the split form, and then applying the strong
-  -- congruence theorem with the support bound above.
-  apply le_iff_exists_add.mp at HN
-  rcases HN with ⟨ diff, Hdiff ⟩
-  subst Hdiff
-  rw [probWhileCut_probWhileSplit_zero]
-  rw [probWhileCut_probWhileSplit_zero]
-
-  -- Turn into a sequence of nested probWhileSplits
-
-
-  -- Re-evaluate: what does this split actually equal?
-  -- Is it
-  --    - last element of the outermost split?
-  --    - the first element of the continuation?
-  -- Which do I want it to be?
-  -- How do I specify that?
-
-  -- Intuition says either might be good
-  -- FRIDAY: Finish lemma about the support of probWhileSplit with True conditional
-
-
-  conv =>
-    lhs
-    enter [4]
-    rw [add_assoc, add_comm]
-  rw [probWhileSplit_add_l]
-  have SC1 :  ∀ (C_1 D : List ℤ), C_1.length < D.length + 1 → probWhileSplit C (@privMax_eval_alt_F dps ε₁ ε₂) (fun x => probZero) (1 + diff) C_1 D = 0 := by
-    intro C1 D HL
-
-
-    -- FIXME Might not be provable sadly
-
-
-    sorry
-  rw [privMax_eval_split_supp_bound' _ _ _ _ _ SC1 (by simp)]
-  conv =>
-    rhs
-    enter [4]
-    rw [add_assoc, add_comm]
-    rw [add_comm B.length]
-    rw [<- add_assoc]
-  rw [probWhileSplit_add_l]
-  have SC2 : ∀ (C_1 D : List ℤ), C_1.length < D.length + 1 → probWhileSplit C (@privMax_eval_alt_F dps ε₁ ε₂) (fun x => probZero) (diff + 1 + 1) C_1 D = 0 := by
-    sorry
-  conv =>
-    rhs
-    rw [privMax_eval_split_supp_bound' _ _ _ _ _ SC2 (by simp)]
-
-  -- Strong congruence and the support equation for the true eqn makes progress????
-  sorry
-
-
-/--
-privMax_eval_alt equals its closed form
--/
-lemma privMax_eval_alt_loop_cut_closed {dps : DPSystem ℕ} :
-    @privMax_eval_alt_loop_cut dps ε₁ ε₂ l τ N h = @privMax_eval_alt_loop_cut_step dps ε₁ ε₂ l τ N h := by
-
-  unfold privMax_eval_alt_loop_cut_step
-  split
-  · -- Below the step
-    unfold privMax_eval_alt_loop_cut
-    apply privMax_eval_cut_supp_bound'
-    simp
-    linarith
-  · -- Above the step
-    rename_i h
-
-    sorry
-
-
-    -- -- Equal to the step point
-    -- cases Classical.em (N = h.length)
-    -- · rename_i Hn
-    --   subst Hn
-    --   sorry
-    --   -- rfl
-    -- · -- Greater than the step point
-
-    --   -- Cleanup context
-    --   rename_i H1 H2
-    --   have H3 : h.length < N := by
-    --     apply lt_of_not_ge
-    --     intro HK
-    --     apply GE.ge.le at HK
-    --     apply LE.le.eq_or_lt at HK
-    --     cases HK <;> simp_all
-    --   clear H1 H2
-
-    --   induction N
-    --   · exfalso
-    --     simp at H3
-    --   rename_i N' IH
-
-    --   cases Classical.em (N' = h.length)
-    --   · simp_all
-    --     simp [privMax_eval_alt_loop_cut]
-    --     -- The real base case
-    --     -- Should be basically the same as the other argument though
-    --     -- Just can't/don't need to rewrite with the IH
-    --     -- unfold privMax_eval_alt_loop_cut
-    --     -- symm
-    --     -- apply privMax_eval_cut_const_ind
-    --     -- sorry
-    --     -- rfl
-    --   rw [<- IH ?G1]
-    --   case G1 =>
-    --     apply Nat.lt_add_one_iff.mp at H3
-    --     apply LE.le.eq_or_lt at H3
-    --     cases H3 <;> simp_all
-
-    --   unfold privMax_eval_alt_loop_cut
-    --   symm
-    --   apply privMax_eval_cut_const_ind
-    --   --  OK
-    --   sorry
-    --   -- linarith
-
-
-
-
-/--
-The first reduction: Evaluate each point using a finite number of iterates
--/
-def privMax_eval_alt_cut {dps : DPSystem ℕ} (ε₁ ε₂ : ℕ+) (l : List ℕ) : SLang ℕ := (fun N =>
-  (do
-    let τ <- @privNoiseZero dps ε₁ (2 * ε₂)
-    let final_history <- @privMax_eval_alt_loop_cut dps ε₁ ε₂ l τ (N + 2)
-    return final_history.length - 1) N)
-
-/-
-The main program equals the cut program
--/
--- lemma privMax_eval_alt_loop_limit :
-
-lemma privMax_reduction_1 (ε₁ ε₂ : ℕ+) (l : List ℕ) :
-    @privMax_eval_alt dps ε₁ ε₂ l = @privMax_eval_alt_cut dps ε₁ ε₂ l := by
-  -- Want to show that the eval (unbounded at each point) equals the cut version (cut to N at each point)
-  apply SLang.ext
-  intro N
-  simp [privMax_eval_alt, privMax_eval_alt_cut]
-  apply tsum_congr
-  intro τ
-  congr
-  apply funext
-  intro returned_hist
-  split <;> try simp
-  rename_i Hreturned_hist
-  simp [privMax_eval_alt_loop, privMax_eval_alt_loop_cut]
-
-  -- Apply probWhile limit lemma
-  apply probWhile_apply
-  apply (@tendsto_atTop_of_eventually_const _ _ _ _ _ _ _ (N + 2))
-
-  -- Prove that probWhileCut is eventually constant
-  intro later_cutoff Hlep
-  rw [<- Nat.add_sub_cancel' Hlep]
-
-
-  -- Change to closed form
-  generalize Hd : (later_cutoff - (N + 1)) = d
-  cases d
-  · simp_all
-    -- OK as long as returned_hist is nonepty, which is always is.
-    sorry
-
-
-  rename_i d'
-
-
-  have H := @privMax_eval_alt_loop_cut_closed
-  unfold privMax_eval_alt_loop_cut at H
-  rw [H]
-
-  -- conv =>
-  --   enter [1, 3]
-  --   rw [add_comm]
-  --   rw [<- add_assoc]
-  --   enter [1]
-  --   rw [add_comm]
-  -- rw [H]
-  -- rename_i d'
-
-  -- rw [privMax_eval_alt_loop_cut_step, privMax_eval_alt_loop_cut_step]
-  -- clear H
-  sorry
-
-
-
-/-
-## Reduction 2: The bounded history-tracking version is the same as a predicate on eager presample
--/
-
--/
-/--
-Sample N noised values. Always returns a list of length N.
--/
-def privMax_sampN {dps : DPSystem ℕ} (ε₁ ε₂ : ℕ+) (N : ℕ) : SLang { v : List ℤ // v.length = N } :=
-  match N with
-  | Nat.zero => probPure ⟨ [], by simp ⟩
-  | Nat.succ N' => do
-      let v <- @privNoiseZero dps ε₁ (4 * ε₂)
-      let r <- @privMax_sampN dps ε₁ ε₂ N'
-      probPure ⟨ r.1 ++ [v], by cases r; simp ; trivial ⟩
-
-/-
-def initDep {N : ℕ} (l : List T) (_ : l.length = N.succ) : List T :=
-  match l with
-  | [_] => []
-  | (v :: h1 :: hs) => v :: @initDep _ (hs.length) (h1 :: hs) (by simp)
-
-lemma initDep_append_singleton {N : ℕ} (l : List T) (vk : T) (Hl : (l ++ [vk]).length = N.succ) :
-    @initDep T N (l ++ [vk]) Hl = l := by
-  revert N
-  induction l
-  · simp [initDep]
-  rename_i h t IH
-  cases t <;> simp_all [initDep]
-
-
-
-/--
-Sample N+1 noise values upfront. Return (N+1) when the first N noised prefix
-sums are less than τ, and the N+1st noised prefix sum exceeds τ.
--/
-def privMax_presample {dps : DPSystem ℕ} (ε₁ ε₂ : ℕ+) (l : List ℕ) : SLang ℕ :=
-(fun N =>
-  (do
-    let τ <- @privNoiseZero dps ε₁ (2 * ε₂)
-    let history <- @privMax_sampN dps ε₁ ε₂ N.succ
-    if (¬ privMax_eval_alt_cond l τ history.1) ∧ (privMax_eval_alt_cond l τ (@initDep ℤ N history.1 (by cases history ; simp ; trivial )) )
-      then probPure N
-      else probZero)
-  N)
-
-
-
-lemma privMax_reduction_2 {dps : DPSystem ℕ} (ε₁ ε₂ : ℕ+) (l : List ℕ)  :
-    @privMax_eval_alt_cut dps ε₁ ε₂ l = @privMax_presample dps ε₁ ε₂ l := by
-  -- Evaluate the identical preludes
-  unfold privMax_presample
-  unfold privMax_eval_alt_cut
-  apply SLang.ext
-  intro N
-  simp only [bind]
-  congr 1
-  apply funext
-  intro τ
-
-  simp [privMax_eval_alt_loop_cut]
-  induction N
-  · simp [privMax_sampN]
-    simp [probWhileCut, probWhileFunctional]
-    conv =>
-      lhs
-      simp [privMax_eval_alt_cond]
-      simp [privMax_eval_alt_F]
-    apply probBind_congr_strong
-    intro v0 Hv0
-    apply SLang.ext
-    intro v
-    simp
-
-    simp [initDep]
-    simp [privMax_eval_alt_cond]
-
-    symm
-    split <;> symm
-    · have Hfin : (∑' (a : List ℤ), if v = a.length - 1 then probPure [v0] a else 0) = probPure 0 v := by
-        simp
-        split
-        · rename_i h
-          subst h
-          rw [ENNReal.tsum_eq_add_tsum_ite [v0]]
-          simp
-          conv =>
-            lhs
-            enter [2]
-            rw [ENNReal.tsum_eq_zero.mpr]
-            · skip
-            · exact by
-                intro i
-                split <;> simp
-          simp
-        · apply ENNReal.tsum_eq_zero.mpr
-          intro _
-          simp
-          intro _ _
-          simp_all
-      sorry
-      -- conv =>
-      -- enter [1, 1, a]
-      -- split
-      -- · exfalso
-      --   linarith
-      -- · apply Hfin
-    · sorry
-      -- simp
-      -- intro i Hv
-      -- split
-      -- · simp
-      -- · exfalso
-      --   aesop
-
-  · rename_i N' IH
-    -- I want to unfold one iteration from both sides, but that means I should
-    -- generalize over initial condition from [] to A
-    sorry
-
-
-/-
-## Reduction 3: Separate the random samples we will view as deterministic, from the random samples for the DP proof.
--/
-
-
--/
-
-def privMax_presample_sep_det {dps : DPSystem ℕ} (ε₁ ε₂ : ℕ+) (N : ℕ) : SLang { v : List ℤ // v.length = N} :=
-  @privMax_sampN dps ε₁ ε₂ N
-
-
-def privMax_presample_sep {dps : DPSystem ℕ} (ε₁ ε₂ : ℕ+) (l : List ℕ) : SLang ℕ :=
-(fun N =>
-  (do
-    -- Part we will parameterize over (ie. using tsum_congr)
-    let history <- @privMax_presample_sep_det dps ε₁ ε₂ N
-
-    -- Part which includes the randomness in the proof (τ and the final sample)
-    let τ <- @privNoiseZero dps ε₁ (2 * ε₂)
-    let vk <- @privNoiseZero dps ε₁ (4 * ε₂)
-    if (¬ privMax_eval_alt_cond l τ (history.1 ++ [vk])) ∧ (privMax_eval_alt_cond l τ history.1)
-      then probPure N
-      else probZero)
-  N)
-
-
-
-/--
-Simpler bijection lemma which ignores the support (makes for much easier fn definitions)
--/
-lemma tsum_eq_tsum_of_bij {α : Type u_1} {β : Type u_2} {γ : Type u_3} [AddCommMonoid α]
-  [TopologicalSpace α] {f : β → α} {g : γ → α}
-    (i : γ → β)
-    (hi : Function.Injective i)
-    (hf : Function.support f ⊆ Set.range fun (x : ↑(Function.support g)) => i ↑x)
-    (hfg : ∀ (x : γ), f (i x) = g x) :
-  ∑' (x : β), f x = ∑' (y : γ), g y := by
-  apply tsum_eq_tsum_of_ne_zero_bij (fun x => i x)
-  · simp [Function.Injective]
-    exact fun a _ a_1 _ a_2 => hi a_2
-  · trivial
-  · simp_all
-
-/-
-def sum_lem_split_lemma_i (N : ℕ) (x : { v : List T // v.length = N } × T) : { v : List T // v.length = N + 1 } :=
-  let ⟨ hist, vk ⟩ := x
-  ⟨ hist ++ [vk], by cases hist ; simp; trivial ⟩
-
-
-lemma splitting_list_lemma {N : ℕ} (hist : List T) (Hhist : hist.length = N + 1) :
-    ∃ vr, ∃ l : List T, hist = l ++ [vr] := by
-  revert N
-  induction hist
-  · simp_all
-  · rename_i hh ht IH
-    cases ht
-    · simp
-      exists hh
-      exists []
-    intro N Hl
-    simp at Hl
-    rename_i hh1 hh2
-    have IH := @IH (hh2.length) ?G1
-    case G1 => simp_all
-    rcases IH with ⟨ a, ⟨ b, c ⟩ ⟩
-    exists a
-    exists (hh :: b)
-    simp [c]
-
-
-lemma sum_len_split_lemma (N : ℕ) (f : { v : List T // v.length = N + 1 } -> ENNReal) :
-    ∑' (a : { v : List T // v.length = N + 1 }), f a =
-    ∑' (a : { v : List T // v.length = N}), ∑'(b : T), f ⟨ a ++ [b], (by cases a; simp; trivial) ⟩ := by
-  rw [← ENNReal.tsum_prod]
-  apply tsum_eq_tsum_of_bij  (sum_lem_split_lemma_i N)
-  · simp [Function.Injective]
-    simp [sum_lem_split_lemma_i]
-    intros _ _ _ _ _ _ H
-    have _ := List.append_inj_left' H
-    simp_all
-  · simp [Function.support]
-    apply Set.setOf_subset.mpr
-    intro x H
-    simp [Set.range]
-    rcases x with ⟨ hist, Hhist ⟩
-    rcases (splitting_list_lemma hist Hhist) with ⟨ a, ⟨ b, c ⟩ ⟩
-    exists b
-    exists ?G1
-    case G1 =>
-      subst c
-      simp at Hhist
-      trivial
-    exists a
-    subst c
-    apply And.intro
-    · trivial
-    · simp [sum_lem_split_lemma_i]
-  · intro x
-    congr 1
-
-
-lemma privMax_reduction_3 {dps : DPSystem ℕ} (ε₁ ε₂ : ℕ+) (l : List ℕ) :
-    @privMax_presample dps ε₁ ε₂ l = @privMax_presample_sep dps ε₁ ε₂ l := by
-  unfold privMax_presample
-  unfold privMax_presample_sep
-  unfold privMax_presample_sep_det
-  simp
-  apply funext
-  intro N
-
-  -- Commute out τ and cancel
-  conv =>
-    enter [2, 1, a]
-    rw [<- ENNReal.tsum_mul_left]
-    enter [1, i]
-    rw [<- mul_assoc]
-    enter [1]
-    rw [mul_comm]
-  conv =>
-    enter [2, 1, a, 1, b]
-    rw [mul_assoc]
-  rw [ENNReal.tsum_comm]
-  conv =>
-    enter [2, 1, a]
-    rw [ENNReal.tsum_mul_left]
-  apply tsum_congr
-  intro τ
-  congr 1
-
-  -- Separate the sums
-  rw [sum_len_split_lemma N]
-  conv =>
-    rhs
-    enter [1, i]
-    rw [<- ENNReal.tsum_mul_left]
-  apply tsum_congr
-  intro history
-  apply tsum_congr
-  intro vk
-
-  -- Simplify away the conditional
-  rcases history with ⟨ history, Hhistory ⟩
-  simp
-  conv =>
-    enter [1, 2]
-    rw [initDep_append_singleton]
-  rw [<- mul_assoc]
-  congr 1
-
-  -- Separate the indicator
-  simp [privMax_sampN]
-  have H (a : ℤ) (b : { v // v.length = N }) :
-       (if history ++ [vk] = ↑b ++ [a] then @privMax_sampN dps ε₁ ε₂ N b else 0) =
-       (if history = ↑b then 1 else 0) * (if vk = a then 1 else 0) * (@privMax_sampN dps ε₁ ε₂ N b) := by
-    symm
-    split <;> try simp_all
-    apply eq_ite_iff.mpr
-    right
-    simp
-    intro HK
-    rename_i h
-    apply h
-    exact List.append_inj_left' HK rfl
-  conv =>
-    enter [1, 1, a, 2, 1, b]
-    rw [H]
-  clear H
-
-  -- Move the a indicator to the outside
-  conv =>
-    enter [1, 1, a, 2, 1, b]
-    rw [mul_comm]
-    rw [<- mul_assoc]
-    rw [mul_comm]
-  conv =>
-    enter [1, 1, a]
-    rw [ENNReal.tsum_mul_left]
-    rw [<- mul_assoc]
-    rw [mul_ite, mul_zero, mul_one]
-
-  rw [<- @tsum_subtype_eq_of_support_subset _ _ _ _ _ { v : ℤ | v = vk } ?G1]
-  case G1 =>
-    simp [Function.support]
-  simp
-  rw [ENNReal.tsum_eq_add_tsum_ite ⟨vk, rfl⟩]
-  simp
-  conv =>
-    lhs
-    enter [2]
-    rw [ENNReal.tsum_eq_zero.mpr
-       (by
-         intro i
-         split <;> simp_all
-         intro H
-         exfalso
-         rename_i H'
-         apply H'
-         subst Hhistory
-         simp_all only [Subtype.coe_eta, not_true_eq_false])]
-    · skip
-  simp
-  rw [mul_comm]
-  congr 1
-
-  -- Same for the other indicator
-  rw [<- @tsum_subtype_eq_of_support_subset _ _ _ _ _ { v : { v // v.length = N } | v = ⟨ history, Hhistory ⟩ } ?G1]
-  case G1 =>
-    simp [Function.support]
-    intros
-    symm
-    trivial
-  rw [ENNReal.tsum_eq_add_tsum_ite ⟨⟨history, Hhistory⟩, rfl⟩]
-  simp
-  rw [ENNReal.tsum_eq_zero.mpr]
-  · simp
-  simp
-
-
-
--/
-def privMax_presample_sep_normalizes : HasSum (@privMax_presample_sep dps ε₁ ε₂ l) 1 := by
-  sorry
-  -- rw [<- privMax_reduction_3]
-  -- rw [<- privMax_reduction_2]
-  -- rw [<- privMax_reduction_1]
-  -- rw [<- privMax_reduction_0]
-  -- exact privMaxPMF_normalizes
-
-
--- To express differential privacy, we need pricMax_presample_sep to be a PMF
-def privMax_presample_sep_PMF {dps : DPSystem ℕ} (ε₁ ε₂ : ℕ+) (l : List ℕ) : PMF ℕ :=
-  ⟨ @privMax_presample_sep dps ε₁ ε₂ l, privMax_presample_sep_normalizes ⟩
-
+def privMax_presample_PMF {dps : DPSystem ℕ} (ε₁ ε₂ : ℕ+) (l : List ℕ) : PMF ℕ :=
+  ⟨ @privMax_presample dps ε₁ ε₂ l, @privMax_presample_normalizes dps ε₁ ε₂ l⟩
 
 end SLang
