SampCert/DifferentialPrivacy/Queries/UnboundedMax/Pure.lean
@@ -40,7 +40,7 @@ lemma tsum_shift_lemma (f : ℤ -> ENNReal) (Δ : ℤ) : ∑'(t : ℤ), f t = �
 /--
 Reduced, history-aware, presampled, separated program  is (ε₁/ε₂)-DP
 -/
-lemma privMax_reduct_PureDP {ε₁ ε₂ : ℕ+} : PureDP (@privMax_presample_sep_PMF PureDPSystem ε₁ ε₂) (ε₁ / ε₂) := by
+lemma privMax_reduct_PureDP {ε₁ ε₂ : ℕ+} : PureDP (@privMax_presample_PMF PureDPSystem ε₁ ε₂) (ε₁ / ε₂) := by
   -- Transform into inequality
   simp [PureDP]
   apply singleton_to_event
@@ -53,53 +53,53 @@ lemma privMax_reduct_PureDP {ε₁ ε₂ : ℕ+} : PureDP (@privMax_presample_se
   case G2 =>
     left
     apply PMF.apply_ne_top
-  unfold privMax_presample_sep_PMF
+  unfold privMax_presample_PMF
   simp [DFunLike.coe, PMF.instFunLike]
 
-  -- Execute the deterministic part
-  simp [privMax_presample_sep]
-  rw [<- ENNReal.tsum_mul_left]
-  apply ENNReal.tsum_le_tsum
-  intro history
-  conv =>
-    enter [2]
-    rw [<- mul_assoc]
-    enter [1]
-    rw [mul_comm]
-  conv =>
-    enter [2]
-    rw [mul_assoc]
-  apply (ENNReal.mul_le_mul_left ?G1 ?G2).mpr
-  case G1 =>
-    -- privMax_presample_sep_det can sample all n-length histories
-    -- Could also reduce this away by conditioning if an issue
-    sorry
-  case G2 =>
-    -- wf
-    sorry
-  rcases history with ⟨ history, Hhistory ⟩
-  simp only []
+  -- -- Execute the deterministic part
+  -- simp [privMax_presample_sep]
+  -- rw [<- ENNReal.tsum_mul_left]
+  -- apply ENNReal.tsum_le_tsum
+  -- intro history
+  -- conv =>
+  --   enter [2]
+  --   rw [<- mul_assoc]
+  --   enter [1]
+  --   rw [mul_comm]
+  -- conv =>
+  --   enter [2]
+  --   rw [mul_assoc]
+  -- apply (ENNReal.mul_le_mul_left ?G1 ?G2).mpr
+  -- case G1 =>
+  --   -- privMax_presample_sep_det can sample all n-length histories
+  --   -- Could also reduce this away by conditioning if an issue
+  --   sorry
+  -- case G2 =>
+  --   -- wf
+  --   sorry
+  -- rcases history with ⟨ history, Hhistory ⟩
+  -- simp only []
 
 
-  -- The n = 0 case is special
-  -- We can't define G when n = 0 (there is nothing to take the max over)
-  -- So we need a different change of variables, I think
-  cases n
-  · simp_all
-    conv =>
-      congr
-      · enter [1, a, 2, 1, b]
-        simp [privMax_eval_alt_cond]
-        simp [G]
-      · enter [2, 1, a, 2, 1, b]
-        simp [privMax_eval_alt_cond]
-        simp [G]
+  -- -- The n = 0 case is special
+  -- -- We can't define G when n = 0 (there is nothing to take the max over)
+  -- -- So we need a different change of variables, I think
+  -- cases n
+  -- · simp_all
+  --   conv =>
+  --     congr
+  --     · enter [1, a, 2, 1, b]
+  --       simp [privMax_eval_alt_cond]
+  --       simp [G]
+  --     · enter [2, 1, a, 2, 1, b]
+  --       simp [privMax_eval_alt_cond]
+  --       simp [G]
 
-    -- Can get away with no COV for τ, I think
+  --   -- Can get away with no COV for τ, I think
 
 
 
-    sorry
+  sorry
     -- rw [<- ENNReal.tsum_mul_left]
     -- apply ENNReal.tsum_le_tsum
     -- intro τ
@@ -124,19 +124,19 @@ lemma privMax_reduct_PureDP {ε₁ ε₂ : ℕ+} : PureDP (@privMax_presample_se
     -- case G1 => sorry
     -- case G2 => sorry
     -- simp [privMax_eval_alt_cond]
-  rename_i N
+  -- rename_i N
 
-  -- Define the shift for the change of variables
-  -- Might have these backwards
-  let cov_Δτ : ℤ := G l₂ ⟨ history, by linarith ⟩ - G l₁ ⟨ history, by linarith ⟩
-  let cov_Δvk  : ℤ := G l₂ ⟨ history, by linarith ⟩ - G l₁ ⟨ history, by linarith ⟩ + exactDiffSum N l₁ - exactDiffSum N l₂
-  conv =>
-    lhs
-    rw [tsum_shift_lemma _ cov_Δτ]
-    enter [1, t]
-    rw [tsum_shift_lemma _ cov_Δvk]
+  -- -- Define the shift for the change of variables
+  -- -- Might have these backwards
+  -- let cov_Δτ : ℤ := G l₂ ⟨ history, by linarith ⟩ - G l₁ ⟨ history, by linarith ⟩
+  -- let cov_Δvk  : ℤ := G l₂ ⟨ history, by linarith ⟩ - G l₁ ⟨ history, by linarith ⟩ + exactDiffSum N l₁ - exactDiffSum N l₂
+  -- conv =>
+  --   lhs
+  --   rw [tsum_shift_lemma _ cov_Δτ]
+  --   enter [1, t]
+  --   rw [tsum_shift_lemma _ cov_Δvk]
 
-  sorry
+  -- sorry
 
 
 
@@ -144,12 +144,12 @@ lemma privMax_reduct_PureDP {ε₁ ε₂ : ℕ+} : PureDP (@privMax_presample_se
 privMax is (ε₁/ε₂)-DP
 -/
 lemma privMax_PureDP {ε₁ ε₂ : ℕ+} : PureDP (@privMaxPMF PureDPSystem ε₁ ε₂) (ε₁ / ε₂) := by
-  apply DPSystem_mech_prop_ext _ _ _ privMax_reduct_PureDP
-  apply funext
-  intro l
-  unfold privMax_presample_sep_PMF
-  unfold privMaxPMF
-  congr
+  -- apply DPSystem_mech_prop_ext _ _ _ privMax_reduct_PureDP
+  -- apply funext
+  -- intro l
+  -- unfold privMax_presample_sep_PMF
+  -- unfold privMaxPMF
+  -- congr
   sorry
   -- rw [privMax_reduction_0]
   -- rw [privMax_reduction_1]
